Fix Free

lean/language.lean
@@ -150,14 +150,26 @@ inductive lang_semantics: IncLoLang.stmt -> LogicType -> IncLoLang.state -> IncL
 
 /-! # Free-/
 
+-- Perhaps invert
 def prop.Free (P: prop): set string :=
-  λ x, ∀ σ v, (P σ ↔ P (σ{x ↦ v}))
+  λ x, ∃ σ v, (P σ ∧ ¬(P (σ{x ↦ v})))
 
-def stmt.Free (C: stmt): set string :=
-  λ x, ∀ σ σ' ty v, lang_semantics C ty σ σ' → lang_semantics C ty (σ{x ↦ v}) (σ'{x ↦ v})
+-- def stmt.Free (C: stmt): set string := // old definition
+--   λ x, ∀ σ σ' ty v, lang_semantics C ty σ σ' → lang_semantics C ty (σ{x ↦ v}) (σ'{x ↦ v})
 
-def expression.Free (e: expression): set string :=
-  λ x, ∀ σ v, e σ = e (σ{x ↦ v})
+def expression.Free (e: expression): set string := 
+  λ x, ∃ σ v, e σ ≠ e (σ{x ↦ v})
+
+def stmt.Free: stmt → set string 
+| stmt.skip                 := {}
+| ([z ↣ e₂])                := {z} ∪ e₂.Free
+| (stmt.non_det_assign z)   := {z}
+| (C₁ ;; C₂)                := (stmt.Free C₁) ∪ (stmt.Free C₂)
+| (C₁ <+> C₂)               := (stmt.Free C₁) ∪ (stmt.Free C₂)
+| (C**)                     := stmt.Free C
+| [loc z . C]               := (stmt.Free C) \ {z}
+| stmt.error                := {}
+| (stmt.assumes P)          := prop.Free P
 
 /-! # Substitute-/
 
@@ -174,7 +186,6 @@ notation P `[` val `//` name `]` :=  prop.substitute name val P
 
 def expression.substitute : string → string → expression → expression
 | x y e := λ σ, e (σ⟨ y // x ⟩)
-
 
 def stmt.substitute : string → string → stmt → stmt
 | x y stmt.skip                 := stmt.skip
@@ -202,32 +213,32 @@ def Mod: stmt -> set string
 | (IncLoLang.stmt.error) := {}
 | (IncLoLang.stmt.local_var x C) := Mod C \ {x}
 
-lemma mod_elem_left_elem_seq (C₁ C₂: stmt) (x: string):
-   x ∈ Mod C₁ → x ∈ Mod (C₁ ;; C₂):=
+lemma mod_elem_left_elem_seq (C₁ C₂: stmt):
+   Mod C₁ ⊆ Mod (C₁ ;; C₂):=
 begin 
   intro h,
   rw Mod,
   finish,
 end
 
-lemma mod_elem_right_elem_seq (C₁ C₂: stmt) (x: string):
-   x ∈ Mod C₂ → x ∈ Mod (C₁ ;; C₂):=
+lemma mod_elem_right_elem_seq (C₁ C₂: stmt):
+   Mod C₂ ⊆ Mod (C₁ ;; C₂):=
 begin 
   intro h,
   rw Mod,
   finish,
 end
 
-lemma mod_elem_left_elem_choice (C₁ C₂: stmt) (x: string):
-   x ∈ Mod C₁ → x ∈ Mod (C₁ <+> C₂):=
+lemma mod_elem_left_elem_choice (C₁ C₂: stmt):
+   Mod C₁ ⊆ Mod (C₁ <+> C₂):=
 begin 
   intro h,
   rw Mod,
   finish,
 end
 
-lemma mod_elem_right_elem_choice (C₁ C₂: stmt) (x: string):
-   x ∈ Mod C₂ → x ∈ Mod (C₁ <+> C₂):=
+lemma mod_elem_right_elem_choice (C₁ C₂: stmt):
+   Mod C₂ ⊆ Mod (C₁ <+> C₂):=
 begin 
   intro h,
   rw Mod,
@@ -273,42 +284,277 @@ begin
   repeat { finish, },
 end
 
-lemma p_thing_free {x v} {P: state -> Prop} :
-  (prop.Free P) ∪ { x } ⊆ prop.Free (P{ x ↣ v }) :=
+/-! ## Free lemmas -/
+
+lemma mod_sub_free (C: stmt):
+  Mod C ⊆ C.Free :=
 begin
-  intros y hx,
-  cases hx,
+  induction C with v r _ C₁ C₂ hC₁ hC₂ C₁ C₂ hC₁ hC₂ _ h,
+  case stmt.skip {
+    rw Mod,
+    exact stmt.skip.Free.empty_subset,
+  },
+  case stmt.assign {
+    rw Mod,
+    rw stmt.Free,
+    exact ({v}: set string).subset_union_left (expression.Free r),
+  },
+  case stmt.non_det_assign {
+    rw Mod,
+    rw stmt.Free,
+  },
+  case stmt.seq {
+    rw Mod,
+    rw stmt.Free,
+    exact set.union_subset_union hC₁ hC₂,
+  },
+  case stmt.choice {
+    rw Mod,
+    rw stmt.Free,
+    exact set.union_subset_union hC₁ hC₂,
+  },
+  case stmt.star {
+    rw Mod,
+    rw stmt.Free,
+    exact h,
+  },
+  case stmt.local_var {
+    rw Mod,
+    rw stmt.Free,
+    exact set.diff_subset_diff_left C_ih,
+  },
+  case stmt.error {
+    rw Mod,
+    rw stmt.Free,
+  },
+  case stmt.assumes {
+    rw Mod,
+    exact (stmt.assumes C).Free.empty_subset,
+  },
+end
+
+lemma not_free_expression {e: expression} {x}: 
+  (¬e.Free x) → ∀ σ v, e σ = e (σ{x ↦ v}) :=
+begin
+  intro h,
+  unfold expression.Free at h,
+  push_neg at h,
+  exact h,
+end
+
+lemma not_free_prop {e: prop} {x}: 
+  (¬e.Free x) → ∀ σ v, e σ ↔ e (σ{x ↦ v}) :=
+begin
+  intro h,
+  unfold prop.Free at h,
+  push_neg at h,
+  intros σ v,
+  split,
+  { exact h σ v, },
   {
-    unfold prop.Free,
-    unfold prop.Free at hx,
-    intros σ v₂,
+    specialize h (σ{x ↦ v}) (σ x),
+    have H: σ{x ↦ v}{x ↦ σ x} = σ, {
+      funext,
+      by_cases x = name',
+      { finish, },
+      { finish, }
+    },
+    rw H at h,
+    exact h,
+  }
+end
+
+lemma free_language_semantics (C: stmt) (x: string):
+  (¬C.Free x) → (∀ σ σ' ty v, lang_semantics C ty σ σ' → lang_semantics C ty (σ{x ↦ v}) (σ'{x ↦ v})) :=
+begin
+  induction C with 
+    y 
+    e y 
+    C₁ C₂ C₁h C₂h 
+    C₁ C₂ C₁h C₂h
+    C Ch
+    z C,
+  case stmt.skip {
+    intros h₁ σ σ' ty v h,
+    cases h,
+    exact lang_semantics.skip,
+  },
+  case stmt.assign {
+    intros h₁ σ σ' ty v h₂,
+    cases h₂,
+    by_cases x = y,
     {
-      unfold p_thing,
-      by_cases x = y,
-      {
-        split,
-        repeat {
-          rw h,
-          rw assign_order_eq,
-          exact id,
-        }
+      exfalso,
+      rw stmt.Free at h₁,
+      apply h₁,
+      left,
+      exact set.mem_singleton_iff.mpr h,
+    },
+    {
+      rw ← state.update,
+      rw assign_order (ne.symm h),
+      -- have H: (λ (name' : string), σ name') = σ, {exact rfl}
+      rw stmt.Free at h₁,
+      have H: e σ = e (σ{x ↦ v}), {
+        by_contra,
+        have H2: x ∈ e.Free, {
+          use σ,
+          use v,
+        },
+        apply h₁,
+        right,
+        exact H2,
       },
-      {
-        rw ← assign_order h,
-        exact (hx (σ{x ↦ v}) v₂), 
-      }
+      rw H,
+      exact lang_semantics.assign,
+    }
+  },
+  case stmt.non_det_assign {
+    intros h₁ σ σ' ty v h₂,
+    cases h₂,
+    by_cases x = y,
+    {
+      exfalso,
+      rw stmt.Free at h₁,
+      apply h₁,
+      exact set.mem_singleton_iff.mpr h,
+    },
+    {
+      rw ← state.update,
+      rw assign_order (ne.symm h),
+      -- have H: (λ (name' : string), σ name') = σ, {exact rfl}
+      rw stmt.Free at h₁,
+
+      exact lang_semantics.non_det_assign h₂_v,
+    }
+  },
+  case stmt.seq {
+    intros h₁ σ σ' ty v h₂,
+    rw stmt.Free at h₁,
+    specialize C₁h (by {
+      by_contra,
+      apply h₁,
+      left,
+      exact h,
+    }),
+    specialize C₂h (by {
+      by_contra,
+      apply h₁,
+      right,
+      exact h,
+    }),
+    cases h₂,
+    {
+      specialize C₁h σ h₂_t LogicType.ok v h₂_H1,
+      specialize C₂h h₂_t σ' ty v h₂_H2,
+      exact lang_semantics.seq_ty C₁h C₂h,
+    },
+    {
+      specialize C₁h σ σ' LogicType.er v h₂_H1,
+      exact lang_semantics.seq_er_1 C₁h,
     },
   },
-  {
+  case stmt.choice {
+    intros h₁ σ σ' ty v h₂,
+    rw stmt.Free at h₁,
+
+    cases h₂,
     {
-      simp at hx,
-      rw hx,
-      unfold prop.Free,
-      intros σ v,
-      split,
-      repeat { unfold p_thing, finish,},
+      specialize C₁h (by {
+        by_contra,
+        apply h₁,
+        left,
+        exact h,
+      }) σ σ' ty v h₂_h,
+      exact lang_semantics.choice_left C₁h,
+    },
+    {
+      specialize C₂h (by {
+        by_contra,
+        apply h₁,
+        right,
+        exact h,
+      }) σ σ' ty v h₂_h,
+      exact lang_semantics.choice_right C₂h,
+    },
+  },
+  case stmt.star {
+    intros h₁ σ σ' ty v h₂,
+    rw stmt.Free at h₁,
+    specialize Ch h₁,
+    cases h₂,
+    use h₂_i,
+    revert σ σ' ty,
+    induction h₂_i,
+    {
+      intros σ σ' ty h,
+      rw repeat at h,
+      cases h,
+      rw repeat,
+      exact lang_semantics.skip,
+    },
+    {
+      intros σ σ' ty h,
+      rw repeat,
+      rw repeat at h,
+      cases h,
+      {
+        exact lang_semantics.seq_ty 
+          (h₂_i_ih σ h_t LogicType.ok h_H1)
+          (Ch h_t σ' ty v h_H2),
+      },
+      { exact lang_semantics.seq_er_1 ( h₂_i_ih σ σ' LogicType.er h_H1 ), }
     }
-  }
+  },
+  case stmt.local_var {
+    intros h₁ σ σ' ty v,
+    rw stmt.Free at h₁,
+    by_cases H: x = z,
+    {
+      cases H,
+      intro h,
+      cases h,
+      rw ← state.update,
+      rw ← state.update,
+      rw assign_order_eq,
+      rw assign_order_eq,
+      exact lang_semantics.local_var h_h,
+    },
+    {
+      have h₂: x ∉ C.Free, {
+        by_contra,
+        apply h₁,
+        split,
+        { exact h, },
+        { 
+          by_contra, 
+          apply H, 
+          exact set.mem_singleton_iff.1 h,
+        },
+      },
+      specialize C_ih h₂,
+      intro h,
+      cases h,
+      rw ← state.update,
+      rw ← state.update,
+      rw assign_order (ne.symm H),
+      rw assign_order (ne.symm H),
+      exact lang_semantics.local_var (C_ih h_s₁ h_s₂ ty v h_h)
+    },
+  },
+  case stmt.error {
+    intros h₁ σ σ' ty v h,
+    cases h,
+    exact lang_semantics.error,
+  },
+  case stmt.assumes {
+    intros h₁ σ σ' ty v h,
+    cases h,
+    rw stmt.Free at h₁,
+    rw prop.Free at h₁,
+    push_neg at h₁,
+    exact lang_semantics.assumes_ok (h₁ σ v h_h),
+  },
 end
 
 lemma assign_semantics {x σ σ' ty} {e: expression}: 
@@ -330,175 +576,206 @@ begin
   repeat { refl },
 end
 
-lemma free_assign {x e}: (stmt.Free ([x ↣ e])) ⊆ (expression.Free e) ∪ {x} :=
+lemma p_thing_free {x v} {P: state -> Prop} :
+  prop.Free (P{ x ↣ v }) ⊆ prop.Free P \ {x} :=
 begin
   intros y hy,
-  by_cases x = y,
+  unfold prop.Free at hy,
+  unfold prop.Free,
+  unfold p_thing at hy,
+  cases hy with σ,
+  use σ{x ↦ v},
+  have Hxy: x ≠ y,
   {
+    by_contra,
     cases h,
-    right,
-    exact set.mem_singleton x,
+    cases hy_h with v,
+    rw assign_order_eq at hy_h_h,
+    finish,
   },
   {
-    left,
-    intros σ v,
-    specialize hy σ (σ{x ↦ e σ}) LogicType.ok v,
-    have H := hy (lang_semantics.assign),
+    cases hy_h with n hn,
+    use n,
+    rw assign_order Hxy,
+    exact hn,
+  },
+  {
+    intro h,
+    finish,
+  },
+end
 
-    have H2 := assign_semantics H,
-    have H3 : (σ{y ↦ v}{x ↦ e (σ{y ↦ v})}) x = e (σ{y ↦ v}), {
-      exact state.update_apply x (e (σ{y ↦ v})) (σ{y ↦ v}),
-    },
 
-    rw ← H3,
+
+-- lemma free_assign {x e}: (stmt.Free ([x ↣ e])) ⊆ (expression.Free e) ∪ {x} :=
+-- begin
+--   intros y hy,
+--   by_cases x = y,
+--   {
+--     cases h,
+--     right,
+--     exact set.mem_singleton x,
+--   },
+--   {
+--     left,
+--     intros σ v,
+--     specialize hy σ (σ{x ↦ e σ}) LogicType.ok v,
+--     have H := hy (lang_semantics.assign),
+
+--     have H2 := assign_semantics H,
+--     have H3 : (σ{y ↦ v}{x ↦ e (σ{y ↦ v})}) x = e (σ{y ↦ v}), {
+--       exact state.update_apply x (e (σ{y ↦ v})) (σ{y ↦ v}),
+--     },
+
+--     rw ← H3,
   
-    have H4 : σ{x ↦ e σ}{y ↦ v} x = e σ, { finish },
-    rw ← H4,
+--     have H4 : σ{x ↦ e σ}{y ↦ v} x = e σ, { finish },
+--     rw ← H4,
 
-    exact congr (eq.symm H2.left) rfl,
-  },
-end
+--     exact congr (eq.symm H2.left) rfl,
+--   },
+-- end
 
-lemma free_assign_2 {x e}: (expression.Free e) \ {x} ⊆ (stmt.Free ([x ↣ e])) :=
-begin
-  intros y hy,
-  intros σ σ' ty v,
-  cases hy,
+-- lemma free_assign_2 {x e}: (expression.Free e) \ {x} ⊆ (stmt.Free ([x ↣ e])) :=
+-- begin
+--   intros y hy,
+--   intros σ σ' ty v,
+--   cases hy,
 
-  specialize hy_left σ v,
-  intro h,
-  cases h,
-  rw ← state.update,
-  rw assign_order (ne.symm hy_right),
-  rw hy_left,
-  exact lang_semantics.assign,
-end
+--   specialize hy_left σ v,
+--   intro h,
+--   cases h,
+--   rw ← state.update,
+--   rw assign_order (ne.symm hy_right),
+--   rw hy_left,
+--   exact lang_semantics.assign,
+-- end
 
-lemma free_non_det_assign {x}: ∀ n, n ∈ (stmt.Free (stmt.non_det_assign x)) :=
-begin
-  unfold stmt.Free,
+-- lemma free_non_det_assign {x}: ∀ n, n ∈ (stmt.Free (stmt.non_det_assign x)) :=
+-- begin
+--   unfold stmt.Free,
 
-  intro n,
-  by_cases n = x,
-  {
-    cases h,
-    intros σ σ' ty v hls,
-    cases hls,
-    have H: (λ (name' : string), ite (name' = x) hls_v (σ name')){x ↦ v} = σ{x ↦ v}{x ↦ v},
-    {
-      funext,
-      by_cases name' = x,
-      { finish, },
-      { finish, }
-    },
-    rw H,
-    exact lang_semantics.non_det_assign v,
-  },
-  {
-    intros σ σ' ty v hls,
-    cases hls,
-    rw ← state.update,
-    rw assign_order (ne.symm h),
-    exact lang_semantics.non_det_assign hls_v,
-  },
-end
+--   intro n,
+--   by_cases n = x,
+--   {
+--     cases h,
+--     intros σ σ' ty v hls,
+--     cases hls,
+--     have H: (λ (name' : string), ite (name' = x) hls_v (σ name')){x ↦ v} = σ{x ↦ v}{x ↦ v},
+--     {
+--       funext,
+--       by_cases name' = x,
+--       { finish, },
+--       { finish, }
+--     },
+--     rw H,
+--     exact lang_semantics.non_det_assign v,
+--   },
+--   {
+--     intros σ σ' ty v hls,
+--     cases hls,
+--     rw ← state.update,
+--     rw assign_order (ne.symm h),
+--     exact lang_semantics.non_det_assign hls_v,
+--   },
+-- end
 
-lemma substitution_rule {ty C y x} {σ σ' : state} (Hyx: y ≠ x) (Hfreey: y ∈ stmt.Free C):
-  lang_semantics C ty (σ) (σ') -> 
-    -- If C can take σ to σ'
-    lang_semantics (C{y // x}) ty (σ⟨ y // x⟩) (σ'⟨ y // x ⟩) :=
-    -- Then C(y/x) can take σ with y set to x's value in σ to σ' with y set to x's value in σ' 
-begin
-  revert ty σ σ',
+-- lemma substitution_rule {ty C y x} {σ σ' : state} (Hyx: y ≠ x) (Hfreey: y ∈ stmt.Free C):
+--   lang_semantics C ty (σ) (σ') -> 
+--     -- If C can take σ to σ'
+--     lang_semantics (C{y // x}) ty (σ⟨ y // x⟩) (σ'⟨ y // x ⟩) :=
+--     -- Then C(y/x) can take σ with y set to x's value in σ to σ' with y set to x's value in σ' 
+-- begin
+--   revert ty σ σ',
 
-  induction C with z e z,
-  case stmt.skip {
-    -- Skip case is trivial as σ = σ'
-    intros _ σ _ h,
-    cases h,
-    exact lang_semantics.skip,
-  },
-  case stmt.assign {
-    intro s,
-    have H := free_assign Hfreey,
-    intros σ σ' hls,
-    cases hls,
-    cases hls,
-    rw stmt.substitute,
-    cases H,
-    { -- case y ∈ Free e
-      sorry,
-    },
-    { -- case y = z
-      sorry,
-    },
-  },
-  case stmt.non_det_assign {
-    intros ty σ σ' hls,
+--   induction C with z e z,
+--   case stmt.skip {
+--     -- Skip case is trivial as σ = σ'
+--     intros _ σ _ h,
+--     cases h,
+--     exact lang_semantics.skip,
+--   },
+--   case stmt.assign {
+--     intro s,
+--     have H := free_assign Hfreey,
+--     intros σ σ' hls,
+--     cases hls,
+--     cases hls,
+--     rw stmt.substitute,
+--     cases H,
+--     { -- case y ∈ Free e
+--       sorry,
+--     },
+--     { -- case y = z
+--       sorry,
+--     },
+--   },
+--   case stmt.non_det_assign {
+--     intros ty σ σ' hls,
 
-    by_cases x = z,
-    {
-      cases h,
-      rw stmt.substitute,
-      cases hls,
-      unfold state.substitute,
-      have H: σ{x ↦ σ y}{x ↦ (σ y)} = (λ (name' : string), ite (name' = x) hls_v (σ name')){x ↦ ite (y = x) hls_v (σ y)}, 
-      {
-        funext,
-        by_cases name' = x,
-        { finish, },
-        { finish, },
-      },
-      rw ← H,
-      exact lang_semantics.non_det_assign (σ y),
-    },
+--     by_cases x = z,
+--     {
+--       cases h,
+--       rw stmt.substitute,
+--       cases hls,
+--       unfold state.substitute,
+--       have H: σ{x ↦ σ y}{x ↦ (σ y)} = (λ (name' : string), ite (name' = x) hls_v (σ name')){x ↦ ite (y = x) hls_v (σ y)}, 
+--       {
+--         funext,
+--         by_cases name' = x,
+--         { finish, },
+--         { finish, },
+--       },
+--       rw ← H,
+--       exact lang_semantics.non_det_assign (σ y),
+--     },
 
-    have H: ∃ v, σ'⟨y//x⟩ = σ⟨y//x⟩{z ↦ v},
-    {
-      cases hls,
-      use hls_v,
-      rw state.substitute,
-      simp,
-      rw ← state.update,
-      rw ← state.update at hls,
+--     have H: ∃ v, σ'⟨y//x⟩ = σ⟨y//x⟩{z ↦ v},
+--     {
+--       cases hls,
+--       use hls_v,
+--       rw state.substitute,
+--       simp,
+--       rw ← state.update,
+--       rw ← state.update at hls,
 
-      by_cases H₂: x = y,
-      {
-        cases H₂,
-        funext,
-        rw if_neg h,
-        rw assign_order h,
-      },
-      {
-        funext,
-        rw if_neg h,
+--       by_cases H₂: x = y,
+--       {
+--         cases H₂,
+--         funext,
+--         rw if_neg h,
+--         rw assign_order h,
+--       },
+--       {
+--         funext,
+--         rw if_neg h,
 
-      }
-      -- ow
+--       }
+--       -- ow
 
 
-    },
+--     },
 
-    have H2: ty = LogicType.ok, { cases hls, refl, },
-    rw H2,
+--     have H2: ty = LogicType.ok, { cases hls, refl, },
+--     rw H2,
 
-    -- | non_det_assign {x s v} :
-    --   lang_semantics (IncLoLang.stmt.non_det_assign x) LogicType.ok s (s{x ↦ v})
+--     -- | non_det_assign {x s v} :
+--     --   lang_semantics (IncLoLang.stmt.non_det_assign x) LogicType.ok s (s{x ↦ v})
 
-    rw stmt.substitute,
-    cases H,
-    rw H_h,
+--     rw stmt.substitute,
+--     cases H,
+--     rw H_h,
 
-    exact lang_semantics.non_det_assign H_w,
-  },
+--     exact lang_semantics.non_det_assign H_w,
+--   },
 
-  sorry,
-  sorry,
-  sorry,
-  sorry,
-  sorry,
-  sorry,
-end
+--   sorry,
+--   sorry,
+--   sorry,
+--   sorry,
+--   sorry,
+--   sorry,
+-- end
 
 end IncLoLang
 
